{"nbformat":4,"nbformat_minor":0,"metadata":{"colab":{"name":"Recursion.ipynb","provenance":[],"collapsed_sections":[],"authorship_tag":"ABX9TyMpQci+nUoV4K/iKrGwzXue"},"kernelspec":{"name":"python3","display_name":"Python 3"},"language_info":{"name":"python"}},"cells":[{"cell_type":"markdown","source":["Tower of Hanoi is a mathematical puzzle where we have three rods and $n$ disks. The objective of the puzzle is to move the entire stack to another rod, obeying the following simple rules: \n","\n","- Only one disk can be moved at a time.\n","- Each move consists of taking the upper disk from one of the stacks and placing it on top of another stack i.e. a disk can only be moved if it is the uppermost disk on a stack.\n","- No disk may be placed on top of a smaller disk."],"metadata":{"id":"ZaSyaUjCH9lc"}},{"cell_type":"markdown","source":["- Define a function $f(n, a, b, c)$ where:\n","    - $n$: Number of disks;\n","    - $a$: The starting rod;\n","    - $b$: The temporary rod;\n","    - $c$: The ending rod.\n","\n","    The function $f$ is responsible to print out the steps of moving $n = k$ disks from $a$ to $c$.\n","\n","- We intend to find a recurrence relation of $f$ at step $n=k$ (i.e. $k$ rods). In other words, we seek to find\n","$$\n","f(n=k, a, b, c) = f(n=k-1, a, b, c) \\cdots \n","$$\n","\n","    where at step number $k$, the function $f$ consist of steps made by $k-1, k-2 \\ldots 1$. We see with an example.\n","\n"],"metadata":{"id":"T7mnHvqMIILC"}},{"cell_type":"markdown","source":["- Define rods $A, B, C$.\n","- The base case:\n","    - $f(n=1, a=A, b=B, c=C)$;\n","    - Move $1$ disk from the starting rod $A$ to ending rod $C$ and we are done.\n","    - We will denote this movement as $A \\to C$ in future.\n","- $n = 2$:\n","    - $f(n=2, a=A, b=B, c=C)$;\n","    - $A \\to B$;\n","    - $A \\to C$;\n","    - $B \\to C$\n","    - At this stage, the recursion and induction is not obvious.\n","- $n = 3$:\n","    - $f(n=3, a=A, b=B, c=C)$;\n","    - $A \\to C$;\n","    - $A \\to B$;\n","    - $C \\to B$;\n","    - $A \\to C$ (Base case)\n","    - $B \\to A$;\n","    - $B \\to C$;\n","    - $A \\to C$\n","- Dissect $n=3$:\n","    - One observes that the first **three** steps is defined by $f(n=2, a=A, b=C, c=B)$. Pay attention that $C$ is now our **temporary rod**. In short, the first three steps is to move **the top 2** rods from $A$ to $B$. This is in fact the problem when $n=2$! **Make a mental note that we are acting as if there are only 2 rods here as we are ignoring the bottom most rod for now, this makes sense since moving the top 2 rods is independent of the bottom most rod.**\n","    - Now we are left with the bottom most rod, let us move it to $C$. This is done by calling the base case, or more simply, just $A \\to C$.\n","    - Lastly, we will move the two rods residing in rod $B$ to $C$, and this is also done by calling $f(n=2, a=B, b=A, c=C)$ where $A$ is now our temporary rod! **Be very clear here that we are just treating this problem as if $n=2$.**\n","    - The above steps make sense for me, but I do not see the recursion properly yet. This is because we didn't think \"recursively\" in step $n=2$. Let us go back and take a look.\n","\n","- Going back to $n=2$:\n","    - "],"metadata":{"id":"e-n-ohw0LkBO"}},{"cell_type":"code","source":["def f(n:int, a, b, c):\n","    # if n==0:\n","    #     return \n","    if n==1:\n","        print(\"me\")\n","        print(f\"Move from {a} to {c}\")\n","        return\n","    f(n-1, a=a, b=c, c=b) # r1 = recursive call 1\n","    print(f\"Move from {a} to {c}\") # r2\n","    f(n-1, a=b, b=a, c=c) # r3\n"],"metadata":{"id":"34X6F6kuQWaa"},"execution_count":null,"outputs":[]},{"cell_type":"code","source":["f(n=1,a=\"A\", b=\"B\", c=\"C\")"],"metadata":{"colab":{"base_uri":"https://localhost:8080/"},"id":"sG8pctaBR9Ss","executionInfo":{"status":"ok","timestamp":1651302915839,"user_tz":-480,"elapsed":589,"user":{"displayName":"HONGNAN GAO","userId":"14684257183016239750"}},"outputId":"591b5acc-a717-4a95-e724-7fa977c55b1e"},"execution_count":null,"outputs":[{"output_type":"stream","name":"stdout","text":["me\n","Move from A to C\n"]}]},{"cell_type":"markdown","source":["- $f(n=2, a=A, b=B, c=C)$:\n","    - $f(n=1, a=A, b=C, c=B)$\n","    - This goes to base case, moving $A$ to $B$.\n","    - At r2, we print $A$ to $C$ because at $n=2$, our arguments are still $a=A, b=B, c=C$.\n","    - Then go r3, we have $f(n=1, a=B, b=A, c=C)$ and thus hits base case again which is $B$ to $C$."],"metadata":{"id":"ZHPFz1IpU5yJ"}},{"cell_type":"code","source":["f(n=2,a=\"A\", b=\"B\", c=\"C\")"],"metadata":{"colab":{"base_uri":"https://localhost:8080/"},"id":"RtTo-jm4R8Un","executionInfo":{"status":"ok","timestamp":1651302928130,"user_tz":-480,"elapsed":431,"user":{"displayName":"HONGNAN GAO","userId":"14684257183016239750"}},"outputId":"063073c0-2e50-46f1-c6f8-31c3a1cd0d88"},"execution_count":null,"outputs":[{"output_type":"stream","name":"stdout","text":["me\n","Move from A to B\n","Move from A to C\n","me\n","Move from B to C\n"]}]},{"cell_type":"code","source":["f(n=3,a=\"A\", b=\"B\", c=\"C\")"],"metadata":{"colab":{"base_uri":"https://localhost:8080/"},"id":"dA2td8sHRHoj","executionInfo":{"status":"ok","timestamp":1651302803501,"user_tz":-480,"elapsed":480,"user":{"displayName":"HONGNAN GAO","userId":"14684257183016239750"}},"outputId":"47f9297a-8d21-452a-8024-44d12df1ff23"},"execution_count":null,"outputs":[{"output_type":"stream","name":"stdout","text":["me\n","Move from A to C\n","Move from A to B\n","me\n","Move from C to B\n","Move from A to C\n","me\n","Move from B to A\n","Move from B to C\n","me\n","Move from A to C\n"]}]},{"cell_type":"markdown","source":["- $f(3, a=A, b=B, c=C)$\n","    - Checks if $n=1$ for base case\n","    - calls $f(n=2, a=A, b=C, c=B)$ which we already know the pattern from above example:\n","        - $f(n=1, a=A, b=B, c=C)$ be very careful here, when we reach here the $b$ and $c$ are swapped once more because at the base case we do want to put $A$ to $C$.\n","        - call stack ends and returns, function goes back to $f(n=2, a=A, b=C, c=B)$\n","    - $f(n=2, a=A, b=C, c=B)$: function is released from $r_1$ and goes to $r_2$ which prints move $A \\to B$ and this function is popped;\n","    - Now we go to "],"metadata":{"id":"aFBd0TBeOQaX"}}]}